vm/stdlib/modules/doc/Token.md
@@ -1636,7 +1636,7 @@ Return Token's module address, module name, and type name of <code>TokenType</co
 
 
 
-<pre><code><b>pragma</b> verify = <b>true</b>;
+<pre><code><b>pragma</b> verify = <b>false</b>;
 <b>pragma</b> aborts_if_is_strict = <b>true</b>;
 </code></pre>
 
